Url.lean
@@ -6,3 +6,4 @@ import Url.Record
 import Url.Parser
 import Url.Urlencoded
 import Url.Api
+import Url.Invariant
